src/program_logic/crash_inv.v
@@ -29,48 +29,63 @@ Proof. rewrite /Tok. apply _. Qed.
 Definition ci_staged k E1 E2 P : iProp Σ :=
   (|={E1, ∅}=> |={∅, ∅}▷=>^k |={∅, E2}=> P)%I.
 
-(*
 Lemma wpc_ci_inv s k N E1 E2 e Φ Φc P γ :
-  ↑N ⊆ E1 →
   ↑N ⊆ E2 →
-  staged_inv N γ (ci_staged (((S (S k)))) (E2 ∖ ↑N) (E2 ∖ ↑N) P) ∗
-  WPC e @ s; (S (S k)); E1; (E2 ∖ ↑N) {{ Φ }} {{ Φc }} ⊢
+  staged_inv N γ (ci_staged (((S (S k)))) (∅) (∅) P) ∗
+  WPC e @ s; (S (S k)); E1; E2 {{ Φ }} {{ |={∅, ↑N}=> Φc }} ⊢
   WPC e @ s; (2 * (S (S (S k)))); E1; E2 {{ Φ }} {{ Φc ∗ P }}.
 Proof.
-  iIntros (??) "(#Hinv&H)".
+  iIntros (Hin) "(#Hinv&H)".
   iApply (wpc_strong_mono s s _ _ E1 _ _ with "H"); try auto.
   { lia. }
-  { set_solver. }
   iSplit; first auto.
   iIntros "HΦc".
-  replace (E2 ∖ (E2 ∖ ↑N)) with (↑N: coPset).
+  rewrite difference_diag_L.
+  iMod "HΦc".
   iMod (staged_inv_weak_open with "Hinv") as "H"; auto.
   rewrite /ci_staged.
   iMod (fupd_intro_mask' _ ∅) as "Hclo"; first by set_solver+.
   replace (2 * S (S (S k)) - S (S k)) with (S (S (S (S k)))) by lia.
   iEval (rewrite Nat_iter_S). do 4 iModIntro.
   iEval (rewrite Nat_iter_S). do 2 iModIntro.
-  iMod "Hclo" as "_".
   iApply (step_fupdN_inner_wand with "H"); auto.
   iIntros; by iFrame.
 Qed.
-*)
+
+Lemma wpc_ci_inv' s k N E1 E2 e Φ Φc P γ :
+  ↑N ⊆ E2 →
+  staged_inv N γ (ci_staged (((S (S k)))) (∅) (∅) P) ∗
+  WPC e @ s; (S (S k)); E1; (E2 ∖ ↑N) {{ Φ }} {{ Φc }} ⊢
+  WPC e @ s; (2 * (S (S (S k)))); E1; E2 {{ Φ }} {{ Φc ∗ P }}.
+Proof.
+  iIntros (Hin) "(#Hinv&H)".
+  iApply (wpc_strong_mono s s _ _ E1 _ _ with "H"); try auto.
+  { lia. }
+  { set_solver. }
+  iSplit; first auto.
+  iIntros "HΦc".
+  replace (E2 ∖ (E2 ∖ ↑N)) with (↑N: coPset); last first.
+  { rewrite {1}(union_difference_L _ _ Hin). set_solver. }
+  iMod (staged_inv_weak_open with "Hinv") as "H"; auto.
+  rewrite /ci_staged.
+  iMod (fupd_intro_mask' _ ∅) as "Hclo"; first by set_solver+.
+  replace (2 * S (S (S k)) - S (S k)) with (S (S (S (S k)))) by lia.
+  iEval (rewrite Nat_iter_S). do 4 iModIntro.
+  iEval (rewrite Nat_iter_S). do 2 iModIntro.
+  iApply (step_fupdN_inner_wand with "H"); auto.
+  iIntros; by iFrame.
+Qed.
 
 (*
-Lemma wpc_staged_invariant_aux s k E1 E2 E1' E2' e Φ Φc P Q1 R1 Q2 R2 N γ' :
+Lemma wpc_staged_invariant_aux s k E1 e Φ Φc P Q1 R1 Q2 R2 N γ' :
   ↑N ⊆ E1 →
-  (E2' ⊆ E1') →
-  (E1 ⊆ E1') →
-  (E2' ⊆ E2) →
   □ (Q1 -∗ R1) ∗
   □ (Q2 -∗ R2) ∗
-  staged_inv N γ' (ci_staged (2 * (S (S (S k)))) E1' E2' P) ∗
-  staged_value N γ' (|={E1 ∖ ↑N, ∅}=> |={∅, ∅}▷=>^(S k)
-                     |={∅, E1 ∖ ↑N}=>
-                     Q1 ∗ WPC e @ k; E1 ∖ ↑N;E2 {{ v, (Φ v ∧ |={E1,E2}=> Φc) ∗ P }}{{Φc ∗ P}} ∗ Q2) ⊢
-  |={E1, ∅}=> |={∅, ∅}▷=>^(S (S (S k))) |={∅, E1}=> R1 ∗ WPC e @ s; S (S k); E1; E2 {{ v, Φ v }} {{Φc}} ∗ R2.
+  staged_inv N γ' (ci_staged (2 * ((S (S k)))) ∅ ∅ P) ∗
+  staged_value N γ' (Q1 ∗ WPC e @ k; E1 ∖ ↑N;∅ {{ v, (Φ v ∧ Φc) ∗ P }}{{Φc ∗ P}} ∗ Q2) ⊢
+  |={E1,E1}_(S (2 * S (S k)))=> R1 ∗ WPC e @ s; (2 * S (S k)); E1; ↑N {{ v, Φ v }} {{Φc}} ∗ R2.
 Proof.
-  iIntros (????) "(#HQR1&#HQR2&#Hsi&Hwp)".
+  iIntros (?) "(#HQR1&#HQR2&#Hsi&Hwp)".
   iLöb as "IH" forall (Q1 Q2 R1 R2 e) "HQR1 HQR2".
   destruct (to_val e) as [v|] eqn:Hval.
   {
@@ -78,21 +93,23 @@ Proof.
     iMod (staged_inv_open with "[$]") as "(H&Hclo')".
     { set_solver. }
     iMod (fupd_intro_mask' _ ∅) as "Hclo"; first by set_solver+.
-    iModIntro. rewrite Nat_iter_S. iModIntro. iNext. iModIntro.
+    iModIntro. rewrite Nat_iter_add. iModIntro. iNext. iModIntro.
     rewrite Nat_iter_S.
     iModIntro. iNext.
     iMod "Hclo" as "_".
-    iMod (fupd_intro_mask' _ (E1 ∖ ↑N)) as "Hclo"; first by set_solver+.
-    iMod "H". iModIntro.
-    rewrite Nat_iter_S. iMod "H".  iModIntro. iNext. iMod "H". iModIntro.
-    iApply (step_fupdN_wand with "H").
-    iIntros "H".
-    iMod "H".
+    rewrite Nat_iter_S.
+    iMod (fupd_intro_mask' _ ∅) as "Hclo"; first by set_solver+.
+    iModIntro. iModIntro. iNext.
+
+
+    iModIntro.
+    iApply step_fupdN_later; first reflexivity. iNext.
+    iApply step_fupdN_later; first reflexivity. iNext.
+    iMod "Hclo".
     rewrite wpc_unfold /wpc_pre.
     rewrite wpc_unfold /wpc_pre.
     rewrite Hval. iDestruct "H" as "(HQ1&(H&_)&HQ2)".
     iMod "H" as "(HΦ&HP)".
-    iMod "Hclo".
     iMod ("Hclo'" with "[HP]").
     { iSplitL. iApply "HP". iAlways.
       iIntros. rewrite /ci_staged.
@@ -107,24 +124,17 @@ Proof.
     iSplit.
     - iDestruct "HΦ" as "($&_)". eauto.
     - iDestruct "HΦ" as "(_&HΦ)".
-      iMod "HΦ". iMod (fupd_intro_mask' _ ∅) as "?"; first by set_solver.
-      iModIntro.
-      iApply step_fupdN_later; first by set_solver.
+      iApply step_fupdN_inner_later; first by set_solver.
       repeat iNext. by iFrame.
   }
-  rewrite (Nat_iter_S ((S (S k)))).
+  iEval (rewrite (Nat_iter_S _)).
   iMod (staged_inv_open with "[$]") as "(H&Hclo')".
   { set_solver. }
   iMod (fupd_intro_mask' _ ∅) as "Hclo"; first by set_solver+.
+  rewrite Nat_iter_add.
   rewrite (Nat_iter_S (S k)).
   iModIntro. iModIntro. iNext. iModIntro.
   iModIntro. iNext.
-  iMod "Hclo" as "_".
-  iMod (fupd_intro_mask' _ (E1 ∖ ↑N)) as "Hclo"; first by set_solver+.
-  iMod "H". iModIntro.
-  iApply (step_fupdN_wand with "H").
-  iIntros "H".
-  iMod "H".
   iMod "Hclo" as "_".
   iDestruct "H" as "(HQ1&H&HQ2)".
   iSpecialize ("Hclo'" $! _ with "[H]").
@@ -141,12 +151,12 @@ Proof.
     { reflexivity. }
     { lia. }
     iApply (step_fupdN_wand with "HP").
-    iIntros "HP". iMod "HP". iDestruct "HP" as "((_&HP)&Hclo')".
-    iMod "Hclo'".
-    iApply fupd_mask_weaken; auto.
+    iIntros "HP". iMod "HP". iDestruct "HP" as "(_&HP)".
+    by iFrame.
   }
   iMod "Hclo'".
-  iModIntro.
+  rewrite -Nat_iter_add. iApply step_fupdN_inner_later; first reflexivity.
+  iNext.
   iSplitL "HQ1".
   { iApply "HQR1". eauto. }
   iSplitR "HQ2"; last first.
@@ -158,8 +168,10 @@ Proof.
     { set_solver. }
     iMod (fupd_intro_mask' _ ∅) as "Hclo''".
     { set_solver. }
-    iModIntro. rewrite Nat_iter_S. rewrite Nat_iter_S.
-    iModIntro. iNext. iModIntro. iModIntro. iNext.
+    iModIntro. rewrite Nat_iter_S. 
+    iModIntro. iNext. rewrite Nat_iter_add.
+    rewrite Nat_iter_S.
+    iModIntro. iModIntro. iNext.
     iMod "Hclo''" as "_".
     rewrite wpc_unfold /wpc_pre.
     rewrite Hval. iDestruct "H" as "(H&_)".
@@ -169,48 +181,220 @@ Proof.
     iModIntro.
     iApply (step_fupdN_wand with "H").
     iIntros "H".
-    iMod "H". iModIntro.
+    rewrite right_id Nat_iter_S.
+    iMod "H". iModIntro. iNext.
     iDestruct "H" as "(%&H)".
+    iApply step_fupdN_inner_later; first reflexivity. do 2 iNext.
     iSplitL "".
     { destruct s; eauto. }
     iIntros.
     iMod ("H" with "[//]") as "H".
-    iModIntro. iNext. iMod "H" as "H".
+  iEval rewrite Nat_iter_S.
+  iModIntro. iModIntro. iNext.
+  rewrite Nat_iter_add.
+  iModIntro. iApply (step_fupdN_le (S k)); [ reflexivity | lia |].
+  iApply (step_fupdN_wand with "H"). iIntros "H".
+  rewrite right_id.
+  iEval rewrite Nat_iter_S.
+  do 2 iMod "H". iModIntro. iNext.
+  iMod "H".
+  iMod "H".
+  iModIntro.
+  iApply (step_fupdN_wand with "H"). iIntros "H".
+  iMod "H".
+  iSpecialize ("Hclo'" $! _ with "[H]").
+  { iSplitL "H". iApply "H".
+    iAlways.
+    iIntros "H".
 
-    iMod "Hclo''" as "_".
-    iSpecialize ("Hclo'" $! _ with "[H]").
-    { iSplitL "H". iApply "H".
-      iAlways. iIntros "H".
-      rewrite /ci_staged.
-      replace (2 * S (S (S k))) with (S (S (S k)) + S (S (S k))) by lia.
-      iApply step_fupdN_inner_plus.
-      iMod (fupd_intro_mask' _ (E1 ∖ ↑N)) as "Hclo''".
-      { set_solver. }
-      iMod "H".
-      iModIntro.
-      iApply (step_fupdN_le (S k)); first reflexivity.
-      { lia. }
-      iApply (step_fupdN_wand with "H"). iIntros "H".
-      iMod "H". iMod "Hclo''" as "_".
-      iDestruct "H" as "(_&H&_)".
-      iPoseProof (wpc_crash with "H") as "H".
-      iModIntro.
-      iMod (fupd_intro_mask') as "Hclo"; [| iMod "H"].
-      { set_solver. }
-      iModIntro.
-      iApply (step_fupdN_le (S k)).
-      { reflexivity. }
-      { lia. }
-      iApply (step_fupdN_wand with "H").
-      iIntros "HP". iMod "HP". iDestruct "HP" as "((_&HP)&Hclo')".
-      iMod "Hclo'".
-      iApply fupd_mask_weaken; auto.
-    }
-    iMod "Hclo'". iModIntro.
+    replace (2 * ((S (S k)))) with (S k + (S (S (S k)))) by lia.
+    iApply step_fupdN_inner_plus.
+    iDestruct "H" as "(_&H&_)".
+    iPoseProof (wpc_crash with "H") as "H".
+    iApply (step_fupdN_wand with "H").
+    iIntros "HP". iMod "HP". iModIntro. iApply step_fupdN_inner_later; auto.
+    do 4 iNext. iDestruct "HP" as "(_&$)".
+  }
+  iMod "Hclo'". iClear "Hclo''".
+  iMod (fupd_intro_mask' _ ∅) as "Hclo''"; first by set_solver+.
+  iModIntro. iModIntro. iNext. iMod "Hclo''" as "_".
+  iModIntro.
     iApply ("IH" with "Hclo' [] []").
     { iAlways. iIntros "H". eauto. }
     { iAlways. iIntros "H". iApply (big_sepL_mono with "H").
       iIntros. iApply (wpc_strong_mono' with "[$]"); eauto.
+      lia.
+      rewrite difference_diag_L; auto.
+    }
+  - iIntros.
+    iMod (staged_inv_open with "[$]") as "(H&Hclo')".
+    { set_solver. }
+    rewrite diag_
+    iMod (fupd_intro_mask' _ ∅) as "Hclo''".
+    { set_solver. }
+    iModIntro. rewrite Nat_iter_S. rewrite Nat_iter_S.
+    iModIntro. iNext. iModIntro. iModIntro. iNext.
+    iMod "Hclo''" as "_".
+    rewrite wpc_unfold /wpc_pre.
+    rewrite Hval. iDestruct "H" as "(_&H)".
+    iMod (fupd_intro_mask' _ (E1 ∖ ↑N)) as "Hclo''".
+    { set_solver. }
+    iMod ("H") as "H".
+    iModIntro.
+    iApply (step_fupdN_wand with "H").
+    iIntros "H".
+    iMod "H" as "(($&HP)&$)".
+    eauto.
+Qed.
+
+Lemma wpc_staged_invariant_aux s k E1 e Φ Φc P Q1 R1 Q2 R2 N γ' :
+  ↑N ⊆ E1 →
+  □ (Q1 -∗ R1) ∗
+  □ (Q2 -∗ R2) ∗
+  staged_inv N γ' (ci_staged (2 * ((S (S k)))) ∅ ∅ P) ∗
+  staged_value N γ' (Q1 ∗ WPC e @ k; E1 ∖ ↑N;∅ {{ v, (Φ v ∧ Φc) ∗ P }}{{Φc ∗ P}} ∗ Q2) ⊢
+  |={E1,E1}_(S (2 * S (S k)))=> R1 ∗ WPC e @ s; (2 * S (S k)); E1; ∅ {{ v, Φ v }} {{Φc}} ∗ R2.
+Proof.
+  iIntros (?) "(#HQR1&#HQR2&#Hsi&Hwp)".
+  iLöb as "IH" forall (Q1 Q2 R1 R2 e) "HQR1 HQR2".
+  destruct (to_val e) as [v|] eqn:Hval.
+  {
+    rewrite Nat_iter_S.
+    iMod (staged_inv_open with "[$]") as "(H&Hclo')".
+    { set_solver. }
+    iMod (fupd_intro_mask' _ ∅) as "Hclo"; first by set_solver+.
+    iModIntro. rewrite Nat_iter_add. iModIntro. iNext. iModIntro.
+    rewrite Nat_iter_S.
+    iModIntro. iNext.
+    iMod "Hclo" as "_".
+    rewrite Nat_iter_S.
+    iMod (fupd_intro_mask' _ ∅) as "Hclo"; first by set_solver+.
+    iModIntro. iModIntro. iNext.
+
+
+    iModIntro.
+    iApply step_fupdN_later; first reflexivity. iNext.
+    iApply step_fupdN_later; first reflexivity. iNext.
+    iMod "Hclo".
+    rewrite wpc_unfold /wpc_pre.
+    rewrite wpc_unfold /wpc_pre.
+    rewrite Hval. iDestruct "H" as "(HQ1&(H&_)&HQ2)".
+    iMod "H" as "(HΦ&HP)".
+    iMod ("Hclo'" with "[HP]").
+    { iSplitL. iApply "HP". iAlways.
+      iIntros. rewrite /ci_staged.
+      iApply step_fupdN_inner_later; first auto.
+      iNext. eauto.
+    }
+    iModIntro.
+    iSplitL "HQ1".
+    { by iApply "HQR1". }
+    iSplitR "HQ2"; last first.
+    { by iApply "HQR2". }
+    iSplit.
+    - iDestruct "HΦ" as "($&_)". eauto.
+    - iDestruct "HΦ" as "(_&HΦ)".
+      iApply step_fupdN_inner_later; first by set_solver.
+      repeat iNext. by iFrame.
+  }
+  iEval (rewrite (Nat_iter_S _)).
+  iMod (staged_inv_open with "[$]") as "(H&Hclo')".
+  { set_solver. }
+  iMod (fupd_intro_mask' _ ∅) as "Hclo"; first by set_solver+.
+  rewrite Nat_iter_add.
+  rewrite (Nat_iter_S (S k)).
+  iModIntro. iModIntro. iNext. iModIntro.
+  iModIntro. iNext.
+  iMod "Hclo" as "_".
+  iDestruct "H" as "(HQ1&H&HQ2)".
+  iSpecialize ("Hclo'" $! _ with "[H]").
+  { iSplitL "H". iApply "H".
+    iAlways.
+    iIntros "H".
+    rewrite wpc_unfold /wpc_pre.
+    rewrite Hval. iDestruct "H" as "(_&HP)".
+    rewrite /ci_staged.
+    iMod (fupd_intro_mask') as "Hclo"; [| iMod "HP"].
+    { set_solver. }
+    iModIntro.
+    iApply (step_fupdN_le (S k)).
+    { reflexivity. }
+    { lia. }
+    iApply (step_fupdN_wand with "HP").
+    iIntros "HP". iMod "HP". iDestruct "HP" as "(_&HP)".
+    by iFrame.
+  }
+  iMod "Hclo'".
+  rewrite -Nat_iter_add. iApply step_fupdN_inner_later; first reflexivity.
+  iNext.
+  iSplitL "HQ1".
+  { iApply "HQR1". eauto. }
+  iSplitR "HQ2"; last first.
+  { iApply "HQR2". eauto. }
+  iEval (rewrite wpc_unfold /wpc_pre). rewrite Hval.
+  iSplit.
+  - iIntros.
+    iMod (staged_inv_open with "[$]") as "(H&Hclo')".
+    { set_solver. }
+    iMod (fupd_intro_mask' _ ∅) as "Hclo''".
+    { set_solver. }
+    iModIntro. rewrite Nat_iter_S. 
+    iModIntro. iNext. rewrite Nat_iter_add.
+    rewrite Nat_iter_S.
+    iModIntro. iModIntro. iNext.
+    iMod "Hclo''" as "_".
+    rewrite wpc_unfold /wpc_pre.
+    rewrite Hval. iDestruct "H" as "(H&_)".
+    iMod (fupd_intro_mask' _ (E1 ∖ ↑N)) as "Hclo''".
+    { set_solver. }
+    iMod ("H" with "[$]") as "H".
+    iModIntro.
+    iApply (step_fupdN_wand with "H").
+    iIntros "H".
+    rewrite right_id Nat_iter_S.
+    iMod "H". iModIntro. iNext.
+    iDestruct "H" as "(%&H)".
+    iApply step_fupdN_inner_later; first reflexivity. do 2 iNext.
+    iSplitL "".
+    { destruct s; eauto. }
+    iIntros.
+    iMod ("H" with "[//]") as "H".
+  iEval rewrite Nat_iter_S.
+  iModIntro. iModIntro. iNext.
+  rewrite Nat_iter_add.
+  iModIntro. iApply (step_fupdN_le (S k)); [ reflexivity | lia |].
+  iApply (step_fupdN_wand with "H"). iIntros "H".
+  rewrite right_id.
+  iEval rewrite Nat_iter_S.
+  do 2 iMod "H". iModIntro. iNext.
+  iMod "H".
+  iMod "H".
+  iModIntro.
+  iApply (step_fupdN_wand with "H"). iIntros "H".
+  iMod "H".
+  iSpecialize ("Hclo'" $! _ with "[H]").
+  { iSplitL "H". iApply "H".
+    iAlways.
+    iIntros "H".
+
+    replace (2 * ((S (S k)))) with (S k + (S (S (S k)))) by lia.
+    iApply step_fupdN_inner_plus.
+    iDestruct "H" as "(_&H&_)".
+    iPoseProof (wpc_crash with "H") as "H".
+    iApply (step_fupdN_wand with "H").
+    iIntros "HP". iMod "HP". iModIntro. iApply step_fupdN_inner_later; auto.
+    do 4 iNext. iDestruct "HP" as "(_&$)".
+  }
+  iMod "Hclo'". iClear "Hclo''".
+  iMod (fupd_intro_mask' _ ∅) as "Hclo''"; first by set_solver+.
+  iModIntro. iModIntro. iNext. iMod "Hclo''" as "_".
+  iModIntro.
+    iApply ("IH" with "Hclo' [] []").
+    { iAlways. iIntros "H". eauto. }
+    { iAlways. iIntros "H". iApply (big_sepL_mono with "H").
+      iIntros. iApply (wpc_strong_mono' with "[$]"); eauto.
+      lia.
+      rewrite difference_diag_L; auto.
     }
   - iIntros.
     iMod (staged_inv_open with "[$]") as "(H&Hclo')".
@@ -233,45 +417,19 @@ Proof.
 Qed.
 *)
 
-Lemma wpc_staged_invariant s k E1 E2 E1' E2' e Φ Φc Q P N γ :
+Lemma wpc_staged_invariant s k E1 e Φ Φc Q P N γ :
   ↑N ⊆ E1 →
-  (E2' ⊆ E1') →
-  (E1 ⊆ E1') →
-  (E2' ⊆ E2) →
   to_val e = None →
-  staged_inv N γ (ci_staged (2 * (S (S (S k)))) ∅ ∅ P) ∗
+  staged_inv N γ (ci_staged (2 * (S (S k))) ∅ ∅ P) ∗
   staged_value N γ Q ∗
-  (▷ (Q) -∗ WPC e @ NotStuck; k; (E1 ∖ ↑N); ∅
-                {{ λ v, (Φ v ∧ |={E1,E2}=> Φc) ∗ P}} {{ Φc ∗ P }}) ⊢
-  WPC e @ s; (S (S k)); E1; ∅ {{ Φ }} {{ Φc }}.
+  (Φc ∧ (▷ (Q) -∗ WPC e @ NotStuck; k; (E1 ∖ ↑N); ∅ {{ λ v, (Φ v ∧ Φc) ∗ P}} {{ Φc ∗ P }})) ⊢
+  WPC e @ s; (2 * S (S k)); E1; ∅ {{ Φ }} {{ Φc }}.
 Proof.
-  iIntros (???? Hval) "(#Hinv&Hval&Hwp)".
+  iIntros (? Hval) "(#Hinv&Hval&Hwp)".
   rewrite !wpc_unfold /wpc_pre.
   iSplit; last first.
   {
-    (* Actually, should just force you to prove Φc when using the rule, before
-          you get the later ▷ Q, then this rule is trivial *)
-    admit.
-    (*
-    iAssert (|={E1,E1}_(S (S (S k)))=> |={∅,∅}_(S (S (S k)))=> Φc)%I with "[-]" as "H".
-    {
-    iMod (staged_inv_open with "[$]") as "(H&Hclo)"; first auto.
-    iMod (fupd_intro_mask' _ ∅) as "Hclo'"; first set_solver+.
-    iModIntro.
-    iEval (rewrite Nat_iter_S). iModIntro. iNext.
-    iDestruct ("Hwp" with "[$]") as "(_&H)".
-    iMod "Hclo'".
-    iApply (step_fupdN_le (S k)); first by set_solver+.
-    { lia. }
-    admit.
-    (*
-    iApply (step_fupdN_wand with "H").
-    iIntros "H". iMod "H" as "(($&?)&$)".
-    eauto.
-     *)
-    }
-    admit.
-     *)
+    iDestruct "Hwp" as "(Hwp&_)". iApply step_fupdN_inner_later; try reflexivity. repeat iNext. eauto.
   }
   rewrite Hval.
   iIntros (????) "Hstate".
@@ -282,10 +440,12 @@ Proof.
   iDestruct ("Hwp" with "[$]") as "(Hwp&_)".
   iMod "Hclo'".
   iMod ("Hwp" with "[$]") as "Hwp". iModIntro.
-  iEval (rewrite Nat_iter_S_r).
+  rewrite Nat_iter_add.
+  iEval rewrite Nat_iter_S_r.
   iApply (step_fupdN_wand with "Hwp").
   iIntros "Hwp".
-  iModIntro. iNext. iModIntro.
+  iModIntro. iNext. rewrite right_id. rewrite Nat_iter_S_r.
+  iApply step_fupdN_inner_later; auto. iNext. iNext. iNext. iModIntro.
   iDestruct "Hwp" as "H".
   iMod "H". iModIntro.
   iDestruct "H" as "(%&H)".
@@ -293,38 +453,37 @@ Proof.
   { destruct s; eauto. }
   iIntros.
   iMod ("H" with "[//]") as "H".
-  iModIntro. iNext. iMod "H" as "H".
+  iEval rewrite Nat_iter_S.
+  iModIntro. iModIntro. iNext.
+  rewrite Nat_iter_add.
+  iModIntro. iApply (step_fupdN_le (S k)); try (auto; lia).
+  iApply (step_fupdN_wand with "H"). iIntros "H".
+  rewrite right_id.
+  iEval rewrite Nat_iter_S.
+  do 2 iMod "H". iModIntro. iNext.
+  iMod "H".
+  iMod "H".
+  iModIntro.
+  iApply (step_fupdN_wand with "H"). iIntros "H".
+  iMod "H".
   iSpecialize ("Hclo" $! _ with "[H]").
   { iSplitL "H". iApply "H".
     iAlways.
     iIntros "H".
 
-    replace (2 * S (S (S k))) with (S (S (S k)) + S (S (S k))) by lia.
+    replace (2 * ((S (S k)))) with (S k + (S (S (S k)))) by lia.
     iApply step_fupdN_inner_plus.
-    
-    iMod (fupd_intro_mask' _ (E1 ∖ ↑N)) as "Hclo''".
-    { set_solver. }
-    iMod "H".
-    iModIntro.
-    iApply (step_fupdN_le (S k)); first reflexivity.
-    { lia. }
-    iApply (step_fupdN_wand with "H"). iIntros "H".
-    iMod "H". iMod "Hclo''" as "_".
     iDestruct "H" as "(_&H&_)".
     iPoseProof (wpc_crash with "H") as "H".
-    iModIntro.
-    iMod (fupd_intro_mask') as "Hclo"; [| iMod "H"].
-    { set_solver. }
-    iModIntro.
-    iApply (step_fupdN_le (S k)).
-    { reflexivity. }
-    { lia. }
     iApply (step_fupdN_wand with "H").
-    iIntros "HP". iMod "HP". iDestruct "HP" as "((_&HP)&Hclo')".
-    iMod "Hclo'".
-    iApply fupd_mask_weaken; auto.
+    iIntros "HP". iMod "HP". iModIntro. iApply step_fupdN_inner_later; auto.
+    do 4 iNext. iDestruct "HP" as "(_&$)".
   }
   iMod "Hclo".
+  iMod (fupd_intro_mask' _ ∅) as "Hclo''"; first by set_solver+.
+  iModIntro. iModIntro. iNext. iMod "Hclo''" as "_".
+  iModIntro.
+  iMod (fupd_intro_mask' _ ∅) as "Hclo''"; first by set_solver+.
   iModIntro.
   iApply (wpc_staged_invariant_aux s k E1 E2 E1' E2'
                 _ Φ Φc P
